Proofs wp_rules Jnz

theories/rules/rules_Jnz.v
@@ -2,95 +2,220 @@ From iris.base_logic Require Export invariants gen_heap.
 From iris.program_logic Require Export weakestpre ectx_lifting.
 From iris.proofmode Require Import proofmode.
 From iris.algebra Require Import frac.
-From cap_machine Require Export rules_base.
+From cap_machine Require Export rules_base register_tactics.
 
 Section cap_lang_rules.
   Context `{memG Σ, regG Σ}.
   Context `{MachineParameters}.
   Implicit Types P Q : iProp Σ.
   Implicit Types σ : ExecConf.
-  Implicit Types c : cap_lang.expr. 
+  Implicit Types c : cap_lang.expr.
   Implicit Types a b : Addr.
   Implicit Types r : RegName.
-  Implicit Types v : cap_lang.val. 
+  Implicit Types v : cap_lang.val.
   Implicit Types w : Word.
   Implicit Types reg : gmap RegName Word.
   Implicit Types ms : gmap Addr Word.
 
-  Inductive Jnz_spec (regs: Reg) (dst src: RegName) : Reg → cap_lang.val → Prop :=
-  | Jnz_spec_failure w:
-      regs !! src = Some w →
-      nonZero w = false →
-      incrementPC regs = None →
-      Jnz_spec regs dst src regs FailedV
-  | Jnz_spec_success1 w regs':
-      regs !! src = Some w →
-      nonZero w = false →
-      incrementPC regs = Some regs' →
-      Jnz_spec regs dst src regs' NextIV
-  | Jnz_spec_success2 w w':
-      regs !! src = Some w →
-      regs !! dst = Some w' →
-      nonZero w = true →
-      Jnz_spec regs dst src (<[PC := updatePcPerm w' ]> regs) NextIV.
+  Inductive Jnz_failure (regs: Reg) (dst src: RegName) (mem : gmap Addr Word) :=
+  | Jnz_fail_cond w:
+    regs !! src = Some w →
+    nonZero w = false →
+    incrementPC regs = None →
+    Jnz_failure regs dst src mem
+  | Jnz_fail_bounds w b e a:
+    regs !! src = Some w →
+    nonZero w = true →
+    regs !! dst = Some (WCap IE b e a) ->
+    (withinBounds b e a = false \/ withinBounds b e (a^+1)%a = false) →
+    Jnz_failure regs dst src mem
+  .
 
-  Lemma wp_Jnz Ep pc_p pc_b pc_e pc_a w dst src regs :
+  Inductive Jnz_spec (regs: Reg) (dst src: RegName)
+    (regs' : Reg) (mem : gmap Addr Word) : cap_lang.val → Prop :=
+  | Jnz_spec_failure :
+    Jnz_failure regs dst src mem ->
+    Jnz_spec regs dst src regs' mem FailedV
+
+  | Jnz_spec_success_IE_t wcond b e a wpc widc:
+    regs !! src = Some wcond →
+    regs !! dst = Some (WCap IE b e a) →
+    nonZero wcond = true →
+    withinBounds b e a = true ->
+    withinBounds b e (a^+1)%a = true ->
+    mem !! a = Some wpc ->
+    mem !! (a^+1)%a = Some widc ->
+    regs' = ( <[ idc := widc ]> (<[ PC := wpc ]> regs)) ->
+    Jnz_spec regs dst src regs' mem NextIV
+
+  | Jnz_spec_success_t w w':
+    regs !! src = Some w →
+    regs !! dst = Some w' →
+    nonZero w = true →
+    is_ie_cap w' = false ->
+    regs' = <[PC := updatePcPerm w' ]> regs ->
+    Jnz_spec regs dst src regs' mem NextIV
+
+  | Jnz_spec_success_f w:
+    regs !! src = Some w →
+    nonZero w = false →
+    incrementPC regs = Some regs' →
+    Jnz_spec regs dst src regs' mem NextIV.
+
+  Definition allow_load_map_or_true r (regs : Reg) (mem : gmap Addr Word):=
+    ∃ p b e a,
+      read_reg_inr regs r p b e a ∧
+        if decide
+             (regs !! r = Some (WCap p b e a)
+              /\ withinBounds b e a = true
+              /\ withinBounds b e (a^+1)%a = true)
+        then
+          (∃ w, mem !! a = Some w) /\ (∃ w, mem !! (a^+1)%a = Some w)
+        else True.
+
+  Lemma wp_Jnz Ep pc_p pc_b pc_e pc_a w dst src regs mem :
     decodeInstrW w = Jnz dst src ->
     isCorrectPC (WCap pc_p pc_b pc_e pc_a) →
+
     regs !! PC = Some (WCap pc_p pc_b pc_e pc_a) →
+    (* TODO extract this hypothesis into a definition *)
+    ( forall wdst wsrc,
+        regs !! dst = Some wdst
+        -> is_ie_cap wdst
+        -> regs !! src = Some wsrc
+        -> nonZero wsrc
+        -> is_Some (regs !! idc) /\ allow_load_map_or_true dst regs mem) ->
     regs_of (Jnz dst src) ⊆ dom regs →
-    
-    {{{ ▷ pc_a ↦ₐ w ∗
-        ▷ [∗ map] k↦y ∈ regs, k ↦ᵣ y }}}
+    mem !! pc_a = Some w →
+
+    {{{ (▷ [∗ map] a↦w ∈ mem, a ↦ₐ w) ∗
+          ▷ [∗ map] k↦y ∈ regs, k ↦ᵣ y }}}
       Instr Executable @ Ep
-    {{{ regs' retv, RET retv;
-        ⌜ Jnz_spec regs dst src regs' retv ⌝ ∗
-        pc_a ↦ₐ w ∗
-        [∗ map] k↦y ∈ regs', k ↦ᵣ y }}}.
+      {{{ regs' retv, RET retv;
+          ⌜ Jnz_spec regs dst src regs' mem retv ⌝ ∗
+            ([∗ map] a↦w ∈ mem, a ↦ₐ w) ∗
+            [∗ map] k↦y ∈ regs', k ↦ᵣ y }}}.
   Proof.
-    iIntros (Hinstr Hvpc HPC Dregs φ) "(>Hpc_a & >Hmap) Hφ".
+    iIntros (Hinstr Hvpc HPC HIE Dregs Hmem_pc φ) "(>Hmem & >Hmap) Hφ".
     iApply wp_lift_atomic_head_step_no_fork; auto.
-    iIntros (σ1 ns l1 l2 nt) "Hσ1 /=". destruct σ1; simpl.
-    iDestruct "Hσ1" as "[Hr Hm]".
+    iIntros (σ1 ns l1 l2 nt) "[Hr Hm] /=". destruct σ1; simpl.
     iDestruct (gen_heap_valid_inclSepM with "Hr Hmap") as %Hregs.
-    have ? := lookup_weaken _ _ _ _ HPC Hregs.
-    iDestruct (@gen_heap_valid with "Hm Hpc_a") as %Hpc_a; auto.
-    iModIntro. iSplitR. by iPureIntro; apply normal_always_head_reducible.
+
+    (* Derive necessary register values in dst and src *)
+    pose proof (lookup_weaken _ _ _ _ HPC Hregs).
+    specialize (indom_regs_incl _ _ _ Dregs Hregs) as Hri. unfold regs_of in Hri.
+    feed destruct (Hri src) as [wsrc [H'src Hsrc]]; first set_solver+.
+    feed destruct (Hri dst) as [wdst [H'dst Hdst]]; first set_solver+.
+    clear Hri.
+    (* Derive the PC in memory *)
+    iDestruct (gen_mem_valid_inSepM mem m with "Hm Hmem") as %Hma; eauto.
+
+    iModIntro.
+    iSplitR. by iPureIntro; apply normal_always_head_reducible.
     iNext. iIntros (e2 σ2 efs Hpstep).
     apply prim_step_exec_inv in Hpstep as (-> & -> & (c & -> & Hstep)).
     iIntros "_".
     iSplitR; auto. eapply step_exec_inv in Hstep; eauto.
+    rewrite /exec /= in Hstep.
 
-    specialize (indom_regs_incl _ _ _ Dregs Hregs) as Hri.
-    unfold regs_of in Hri, Dregs.
-    destruct (Hri src) as [wsrc [H'src Hsrc]]. by set_solver+.
-    destruct (Hri dst) as [wdst [H'dst Hdst]]. by set_solver+.
-    unfold exec in Hstep; cbn in Hstep.
-
+    (* Now we start splitting on the different cases in the Jnz spec, and prove them one at a time *)
     destruct (nonZero wsrc) eqn:Hnz; pose proof Hnz as H'nz;
       cbn in Hstep; rewrite Hsrc Hdst /= Hnz in Hstep.
-    { inv Hstep. simplify_pair_eq.
-      iMod ((gen_heap_update_inSepM _ _ PC) with "Hr Hmap") as "[Hr Hmap]"; eauto.
-      iFrame. iApply "Hφ". iFrame. iPureIntro. econstructor 3; eauto. }
+    { (* wsrc is non-zero, destruct on the dst *)
+      destruct (is_ie_cap wdst) eqn:Hwdst.
+      - (* wdst is an IE-cap *)
+        destruct wdst ; cbn in Hwdst; try discriminate.
+        destruct sb as [ p b e a |]; cbn in Hwdst; try discriminate.
+        destruct p; try discriminate ; clear Hwdst.
 
+        (* destruct the bounds *)
+        destruct (decide (withinBounds b e a && withinBounds b e (a ^+ 1)%a)) as
+          [Hbounds%Is_true_true | Hbounds%Is_true_false]
+        ; (rewrite Hbounds /= in Hstep).
+        * (* in bounds, success *)
+          pose proof H'dst as H'dst'.
+          eapply HIE in H'dst';eauto ; clear HIE.
+          destruct H'dst' as [HIDC HaLoad].
+          unfold allow_load_map_or_true in HaLoad.
+          destruct HaLoad as (p' & b' & e' & a' & Hread_reg & HaLoad).
+          unfold read_reg_inr in Hread_reg.
+          rewrite H'dst in Hread_reg.
+          injection Hread_reg ; intros ; subst ; clear Hread_reg.
+
+          case_decide.
+          2: { (* contradiction *)
+            exfalso.
+            apply andb_true_iff in Hbounds.
+            apply H3; split ; auto.
+          }
+          destruct HaLoad as [[wpc Ha] [widc Ha']].
+
+          iDestruct (gen_mem_valid_inSepM mem m a' wpc with "Hm Hmem" ) as %Hma'
+          ; eauto.
+          iDestruct (gen_mem_valid_inSepM mem m (a'^+1)%a widc with "Hm Hmem" ) as %Hma''
+          ; eauto.
+          rewrite Hma' Hma'' /= in Hstep; simplify_pair_eq; simpl.
+          iMod ((gen_heap_update_inSepM _ _ PC wpc) with "Hr Hmap") as "[Hr Hmap]"; eauto.
+          iMod ((gen_heap_update_inSepM _ _ idc widc) with "Hr Hmap") as
+            "[Hr Hmp]" ; eauto.
+          { apply lookup_insert_is_Some'; by right. }
+          iFrame; try iApply "Hφ"; iFrame.
+          apply andb_true_iff in Hbounds ; destruct Hbounds as [Hbounds_a Hbounds_a'].
+          iPureIntro; econstructor; eauto.
+        * (* in bounds, failure *)
+          simplify_pair_eq ; iFrame ; iApply "Hφ"; iFrame.
+          iPureIntro; eapply Jnz_spec_failure ; eapply Jnz_fail_bounds ; eauto.
+          by apply andb_false_iff.
+
+      - (* wdst is not an IE-cap *)
+
+        (* TODO use =match goal with= instead *)
+        rewrite (_ :
+            match wdst with
+            | WCap IE b e a =>
+                if withinBounds b e a && withinBounds b e (a ^+ 1)%a
+                then
+                 m !! a
+                 ≫= (λ wpc : Word,
+                       m !! (a ^+ 1)%a
+                       ≫= (λ widc : Word,
+                             Some (NextI, update_reg (update_reg (r, m) PC wpc) idc widc)))
+                else None
+            | _ => Some (NextI, update_reg (r, m) PC (updatePcPerm wdst))
+            end = Some (NextI, update_reg (r, m) PC (updatePcPerm wdst))) in
+          Hstep.
+        2: {
+        destruct wdst ; cbn in Hwdst; try discriminate; auto.
+        destruct sb as [ p b e a |]; cbn in Hwdst; try discriminate; auto.
+        destruct p; try discriminate ; auto.
+        }
+
+      simplify_pair_eq; simpl.
+      iMod ((gen_heap_update_inSepM _ _ PC) with "Hr Hmap") as "[Hr Hmap]"; eauto.
+      iFrame.
+      iApply "Hφ". iFrame. iPureIntro; econstructor 3; eauto.
+    }
+
+    (* wsrc is zero, destruct on the dst *)
     destruct (incrementPC regs) eqn:HX; pose proof HX as H'X; cycle 1.
     { apply incrementPC_fail_updatePC with (m:=m) in HX.
       eapply updatePC_fail_incl with (m':=m) in HX; eauto.
       rewrite HX in Hstep. inv Hstep.
-      iFrame. iApply "Hφ". iFrame. iPureIntro; econstructor; eauto. }
+      iFrame. iApply "Hφ". iFrame. iPureIntro; econstructor ; econstructor; eauto. }
 
     destruct (incrementPC_success_updatePC _ m _ HX)
       as (p' & g' & b' & e' & a'' & a_pc' & HPC'' & HuPC & ->).
     eapply updatePC_success_incl with (m':=m) in HuPC; eauto. rewrite HuPC in Hstep.
     simplify_pair_eq.
     iMod ((gen_heap_update_inSepM _ _ PC) with "Hr Hmap") as "[Hr Hmap]"; eauto.
-    iFrame. iApply "Hφ". iFrame. iPureIntro. econstructor 2; eauto.
+    iFrame. iApply "Hφ". iFrame. iPureIntro; econstructor 4; eauto.
   Qed.
 
   Lemma wp_jnz_success_jmp E r1 r2 pc_p pc_b pc_e pc_a w w1 w2 :
     decodeInstrW w = Jnz r1 r2 →
     isCorrectPC (WCap pc_p pc_b pc_e pc_a) →
     w2 ≠ WInt 0%Z →
+    is_ie_cap w1 = false ->
 
     {{{ ▷ PC ↦ᵣ WCap pc_p pc_b pc_e pc_a
         ∗ ▷ pc_a ↦ₐ w
@@ -103,28 +228,105 @@ Section cap_lang_rules.
           ∗ r1 ↦ᵣ w1
           ∗ r2 ↦ᵣ w2 }}}.
   Proof.
-    iIntros (Hinstr Hvpc Hne ϕ) "(>HPC & >Hpc_a & >Hr1 & >Hr2) Hφ".
+    iIntros (Hinstr Hvpc Hne Hdst ϕ) "(>HPC & >Hpc_a & >Hr1 & >Hr2) Hφ".
     iDestruct (map_of_regs_3 with "HPC Hr1 Hr2") as "[Hmap (%&%&%)]".
-    iApply (wp_Jnz with "[$Hmap Hpc_a]"); eauto; simplify_map_eq; eauto.
-    by unfold regs_of; rewrite !dom_insert; set_solver+.
-    iNext. iIntros (regs' retv) "(#Hspec & Hpc_a & Hmap)". iDestruct "Hspec" as %Hspec.
+    iDestruct (memMap_resource_1 with "Hpc_a") as "Hmem".
+
+    iApply (wp_Jnz with "[$Hmap $Hmem]"); eauto; simplify_map_eq; eauto.
+    { intros ; simplify_eq. by rewrite Hdst in H6. }
+    { by unfold regs_of; rewrite !dom_insert; set_solver+. }
+    iNext. iIntros (regs' retv) "(#Hspec & Hmem & Hreg)". iDestruct "Hspec" as %Hspec.
 
     assert (nonZero w2 = true).
     { unfold nonZero, Zneq_bool in *.
       repeat case_match; try congruence; subst. exfalso.
       apply Hne. f_equal. by apply Z.compare_eq. }
 
-   destruct Hspec as [ | | ].
-   { exfalso. simplify_map_eq. congruence. }
-   { exfalso. simplify_map_eq. congruence. }
-   { iApply "Hφ". iFrame. simplify_map_eq. rewrite insert_insert.
-     iDestruct (regs_of_map_3 with "Hmap") as "(?&?&?)"; eauto; iFrame. }
+   destruct Hspec as [ X | | | ]
+   ; [destruct X | | | ]
+   ; try (exfalso; simplify_map_eq; congruence).
+    subst regs'; simplify_map_eq.
+    iApply "Hφ".
+    iExtractList "Hreg" [PC; r1; r2] as ["HPC"; "Hr1"; "Hr2"]; iFrame.
+    iDestruct (big_sepM_insert with "Hmem") as "[Hpc_a _]"; auto.
   Qed.
 
-  Lemma wp_jnz_success_jmp2 E r2 pc_p pc_b pc_e pc_a w w2 :
+  (* TODO we need to do more cases where:
+       - r = idc
+       - pc_a = a
+       - pc_a = a+1
+   *)
+  Lemma wp_jnz_success_jmp_IE E r1 r2 pc_p pc_b pc_e pc_a w w' w2 b e a wpc widc :
+    decodeInstrW w = Jnz r1 r2 →
+    isCorrectPC (WCap pc_p pc_b pc_e pc_a) →
+    withinBounds b e a = true ->
+    withinBounds b e (a^+1)%a = true ->
+    w2 ≠ WInt 0%Z →
+
+    {{{ ▷ PC ↦ᵣ WCap pc_p pc_b pc_e pc_a
+          ∗ ▷ idc ↦ᵣ w'
+          ∗ ▷ r1 ↦ᵣ WCap IE b e a
+          ∗ ▷ r2 ↦ᵣ w2
+          ∗ ▷ pc_a ↦ₐ w
+          ∗ ▷ a ↦ₐ wpc
+          ∗ ▷ (a^+1)%a ↦ₐ widc
+    }}}
+      Instr Executable @ E
+      {{{ RET NextIV;
+          PC ↦ᵣ wpc
+          ∗ ▷ idc ↦ᵣ widc
+          ∗ ▷ r1 ↦ᵣ WCap IE b e a
+          ∗ r2 ↦ᵣ w2
+          ∗ ▷ pc_a ↦ₐ w
+          ∗ ▷ a ↦ₐ wpc
+          ∗ ▷ (a^+1)%a ↦ₐ widc
+      }}}.
+  Proof.
+    iIntros (Hinstr Hvpc Hbound_a Hbound_a' Hne ϕ)
+      "(>HPC & >HIDC & >Hr1 & >Hr2 & >Hpc_a & >Ha & >Ha') Hφ".
+    iDestruct (map_of_regs_4 with "HPC HIDC Hr1 Hr2") as "[Hmap (%&%&%&%&%&%)]".
+
+    iDestruct (address_neq with "Ha' Hpc_a") as "%Ha'".
+    iDestruct (address_neq with "Ha Ha'") as "%Hneqa".
+    iDestruct (memMap_resource_2ne_apply with "Hpc_a Ha") as "[Hmem %Ha]".
+    iDestruct (big_sepM_insert with "[Ha' Hmem]") as "Hmem" ; [| iFrame |].
+    by simplify_map_eq.
+
+    iApply (wp_Jnz with "[$Hmap $Hmem]"); eauto; simplify_map_eq; eauto.
+    { intros * Hdst Hdst_IE Hsrc Hsrc_nz ; simplify_eq.
+      split ; auto.
+      unfold allow_load_map_or_true. exists IE, b, e, a.
+      split.
+      unfold read_reg_inr; by simplify_map_eq.
+      case_decide as H' ; auto ; clear H'.
+      split ; eexists ; by simplify_map_eq. }
+    { by unfold regs_of; rewrite !dom_insert; set_solver+. }
+    iNext. iIntros (regs' retv) "(#Hspec & Hmem & Hreg)". iDestruct "Hspec" as %Hspec.
+
+    assert (nonZero w2 = true).
+    { unfold nonZero, Zneq_bool in *.
+      repeat case_match; try congruence; subst. exfalso.
+      apply Hne. f_equal. by apply Z.compare_eq. }
+
+   destruct Hspec as [ X | | | ]
+   ; [destruct X | | | ]
+   ; try (exfalso; simplify_map_eq; congruence)
+   ; simplify_map_eq.
+    { by destruct o as [o | o] ; [rewrite o in Hbound_a | rewrite o in Hbound_a']. }
+    iApply "Hφ".
+    iExtractList "Hreg" [PC; idc ; r1; r2] as ["HPC"; "HIDC" ;"Hr1"; "Hr2"]; iFrame.
+      iDestruct (big_sepM_insert with "Hmem") as "[Ha' Hmem]"; auto ; [ by simplify_map_eq|].
+      iDestruct (big_sepM_insert with "Hmem") as "[Hpc_a Hmem]"; auto ; [ by simplify_map_eq|].
+      iDestruct (big_sepM_insert with "Hmem") as "[Ha _]"; auto.
+      iFrame.
+  Qed.
+
+  (* TODO version fail with IE *)
+  Lemma wp_jnz_success_jmp_same E r2 pc_p pc_b pc_e pc_a w w2 :
     decodeInstrW w = Jnz r2 r2 →
     isCorrectPC (WCap pc_p pc_b pc_e pc_a) →
     w2 ≠ WInt 0%Z →
+    is_ie_cap w2 = false ->
 
     {{{ ▷ PC ↦ᵣ WCap pc_p pc_b pc_e pc_a
         ∗ ▷ pc_a ↦ₐ w
@@ -135,22 +337,28 @@ Section cap_lang_rules.
           ∗ pc_a ↦ₐ w
           ∗ r2 ↦ᵣ w2 }}}.
   Proof.
-    iIntros (Hinstr Hvpc Hne ϕ) "(>HPC & >Hpc_a & >Hr2) Hφ".
+    iIntros (Hinstr Hvpc Hne Hdst ϕ) "(>HPC & >Hpc_a & >Hr2) Hφ".
     iDestruct (map_of_regs_2 with "HPC Hr2") as "[Hmap %]".
-    iApply (wp_Jnz with "[$Hmap Hpc_a]"); eauto; simplify_map_eq; eauto.
-    by unfold regs_of; rewrite !dom_insert; set_solver+.
-    iNext. iIntros (regs' retv) "(#Hspec & Hpc_a & Hmap)". iDestruct "Hspec" as %Hspec.
+    iDestruct (memMap_resource_1 with "Hpc_a") as "Hmem".
+
+    iApply (wp_Jnz with "[$Hmap $Hmem]"); eauto; simplify_map_eq; eauto.
+    { intros * Heq. injection Heq ; intros ; subst ; clear Heq.
+      by rewrite Hdst in H4. }
+    { by unfold regs_of; rewrite !dom_insert; set_solver+. }
+    iNext. iIntros (regs' retv) "(#Hspec & Hmem & Hreg)". iDestruct "Hspec" as %Hspec.
 
     assert (nonZero w2 = true).
     { unfold nonZero, Zneq_bool in *.
       repeat case_match; try congruence; subst. exfalso.
       apply Hne. f_equal. by apply Z.compare_eq. }
 
-   destruct Hspec as [ | | ].
-   { exfalso. simplify_map_eq. congruence. }
-   { exfalso. simplify_map_eq. congruence. }
-   { iApply "Hφ". iFrame. simplify_map_eq. rewrite insert_insert.
-     iDestruct (regs_of_map_2 with "Hmap") as "(?&?)"; eauto; iFrame. }
+   destruct Hspec as [ X | | | ]
+   ; [destruct X | | | ]
+   ; try (exfalso; simplify_map_eq; congruence).
+    subst regs'; simplify_map_eq.
+    iApply "Hφ".
+    iExtractList "Hreg" [PC; r2] as ["HPC"; "Hr2"]; iFrame.
+    iDestruct (big_sepM_insert with "Hmem") as "[Hpc_a _]"; auto.
   Qed.
 
   Lemma wp_jnz_success_jmpPC E pc_p pc_b pc_e pc_a w :
@@ -166,13 +374,22 @@ Section cap_lang_rules.
   Proof.
     iIntros (Hinstr Hvpc ϕ) "(>HPC & >Hpc_a) Hφ".
     iDestruct (map_of_regs_1 with "HPC") as "Hmap".
-    iApply (wp_Jnz with "[$Hmap Hpc_a]"); eauto; simplify_map_eq; eauto.
-    by unfold regs_of; rewrite !dom_insert; set_solver+.
-    iNext. iIntros (regs' retv) "(#Hspec & Hpc_a & Hmap)". iDestruct "Hspec" as %Hspec.
+    iDestruct (memMap_resource_1 with "Hpc_a") as "Hmem".
+    iApply (wp_Jnz with "[$Hmap $Hmem]"); eauto; simplify_map_eq; eauto.
+    { intros * Hcontra; injection Hcontra ; intros ; subst.
+      by apply isCorrectPC_not_ie_cap in Hvpc ; rewrite Hvpc in H3.
+    }
+    { by unfold regs_of; rewrite !dom_insert; set_solver+. }
+    iNext. iIntros (regs' retv) "(#Hspec & Hmem & Hreg)". iDestruct "Hspec" as %Hspec.
 
-   destruct Hspec as [ | | ]; [ by simplify_map_eq .. | ].
-   { iApply "Hφ". iFrame. simplify_map_eq. rewrite insert_insert.
-     iDestruct (regs_of_map_1 with "Hmap") as "?"; eauto; iFrame. }
+   destruct Hspec as [ X | | | ]
+   ; [destruct X | | | ]
+   ; try (exfalso; simplify_map_eq; congruence)
+   ; try (simplify_map_eq; apply isCorrectPC_not_ie_cap in Hvpc ; cbn in Hvpc ; congruence).
+    subst regs'; simplify_map_eq.
+    iApply "Hφ".
+    iExtractList "Hreg" [PC] as ["HPC"]; iFrame.
+    iDestruct (big_sepM_insert with "Hmem") as "[Hpc_a _]"; auto.
   Qed.
 
   Lemma wp_jnz_success_jmpPC1 E r2 pc_p pc_b pc_e pc_a w w2 :
@@ -191,25 +408,35 @@ Section cap_lang_rules.
   Proof.
     iIntros (Hinstr Hvpc Hne ϕ) "(>HPC & >Hpc_a & >Hr2) Hφ".
     iDestruct (map_of_regs_2 with "HPC Hr2") as "[Hmap %]".
-    iApply (wp_Jnz with "[$Hmap Hpc_a]"); eauto; simplify_map_eq; eauto.
-    by unfold regs_of; rewrite !dom_insert; set_solver+.
-    iNext. iIntros (regs' retv) "(#Hspec & Hpc_a & Hmap)". iDestruct "Hspec" as %Hspec.
+    iDestruct (memMap_resource_1 with "Hpc_a") as "Hmem".
+    iApply (wp_Jnz with "[$Hmap $Hmem]"); eauto; simplify_map_eq; eauto.
+    { intros * Hcontra; injection Hcontra ; intros ; subst.
+      by apply isCorrectPC_not_ie_cap in Hvpc ; rewrite Hvpc in H4.
+    }
+    { by unfold regs_of; rewrite !dom_insert; set_solver+. }
+    iNext. iIntros (regs' retv) "(#Hspec & Hmem & Hreg)". iDestruct "Hspec" as %Hspec.
 
     assert (nonZero w2 = true).
     { unfold nonZero, Zneq_bool in *.
       repeat case_match; try congruence; subst. exfalso.
       apply Hne. f_equal. by apply Z.compare_eq. }
 
-   destruct Hspec as [ | | ].
-   { exfalso. simplify_map_eq. congruence. }
-   { exfalso. simplify_map_eq. congruence. }
-   { iApply "Hφ". iFrame. simplify_map_eq. rewrite insert_insert.
-     iDestruct (regs_of_map_2 with "Hmap") as "(?&?)"; eauto; iFrame. }
+
+   destruct Hspec as [ X | | | ]
+   ; [destruct X | | | ]
+   ; try (exfalso; simplify_map_eq; congruence)
+   ; try (simplify_map_eq; apply isCorrectPC_not_ie_cap in Hvpc ; cbn in Hvpc ; congruence).
+    subst regs'; simplify_map_eq.
+    iApply "Hφ".
+    iExtractList "Hreg" [PC; r2] as ["HPC";"Hr2"]; iFrame.
+    iDestruct (big_sepM_insert with "Hmem") as "[Hpc_a _]"; auto.
   Qed.
 
+  (* TODO version with IE *)
   Lemma wp_jnz_success_jmpPC2 E r1 pc_p pc_b pc_e pc_a w w1 :
     decodeInstrW w = Jnz r1 PC →
     isCorrectPC (WCap pc_p pc_b pc_e pc_a) →
+    is_ie_cap w1 = false ->
 
     {{{ ▷ PC ↦ᵣ WCap pc_p pc_b pc_e pc_a
         ∗ ▷ pc_a ↦ₐ w
@@ -220,15 +447,23 @@ Section cap_lang_rules.
           ∗ pc_a ↦ₐ w
           ∗ r1 ↦ᵣ w1 }}}.
   Proof.
-    iIntros (Hinstr Hvpc ϕ) "(>HPC & >Hpc_a & >Hr1) Hφ".
+    iIntros (Hinstr Hvpc Hdst ϕ) "(>HPC & >Hpc_a & >Hr1) Hφ".
     iDestruct (map_of_regs_2 with "HPC Hr1") as "[Hmap %]".
-    iApply (wp_Jnz with "[$Hmap Hpc_a]"); eauto; simplify_map_eq; eauto.
-    by unfold regs_of; rewrite !dom_insert; set_solver+.
-    iNext. iIntros (regs' retv) "(#Hspec & Hpc_a & Hmap)". iDestruct "Hspec" as %Hspec.
+    iDestruct (memMap_resource_1 with "Hpc_a") as "Hmem".
+    iApply (wp_Jnz with "[$Hmap $Hmem]"); eauto; simplify_map_eq; eauto.
+    { intros * Hcontra; injection Hcontra ; intros ; subst.
+      by rewrite Hdst in H4. }
+    { by unfold regs_of; rewrite !dom_insert; set_solver+. }
+    iNext. iIntros (regs' retv) "(#Hspec & Hmem & Hreg)". iDestruct "Hspec" as %Hspec.
 
-   destruct Hspec as [ | | ]; [ by simplify_map_eq .. | ].
-   { iApply "Hφ". iFrame. simplify_map_eq. rewrite insert_insert.
-     iDestruct (regs_of_map_2 with "Hmap") as "(?&?)"; eauto; iFrame. }
+
+   destruct Hspec as [ X | | | ]
+   ; [destruct X | | | ]
+   ; try (exfalso; simplify_map_eq; congruence).
+    subst regs'; simplify_map_eq.
+    iApply "Hφ".
+    iExtractList "Hreg" [PC; r1] as ["HPC";"Hr1"]; iFrame.
+    iDestruct (big_sepM_insert with "Hmem") as "[Hpc_a _]"; auto.
   Qed.
 
   Lemma wp_jnz_success_next E r1 r2 pc_p pc_b pc_e pc_a pc_a' w w1 :
@@ -249,14 +484,20 @@ Section cap_lang_rules.
   Proof.
     iIntros (Hinstr Hvpc Hpc_a' ϕ) "(>HPC & >Hpc_a & >Hr1 & >Hr2) Hφ".
     iDestruct (map_of_regs_3 with "HPC Hr1 Hr2") as "[Hmap (%&%&%)]".
-    iApply (wp_Jnz with "[$Hmap Hpc_a]"); eauto; simplify_map_eq; eauto.
-    by unfold regs_of; rewrite !dom_insert; set_solver+.
-    iNext. iIntros (regs' retv) "(#Hspec & Hpc_a & Hmap)". iDestruct "Hspec" as %Hspec.
+    iDestruct (memMap_resource_1 with "Hpc_a") as "Hmem".
+    iApply (wp_Jnz with "[$Hmap $Hmem]"); eauto; simplify_map_eq; eauto.
+    { intros * _ _ Hcontra Hnz. injection Hcontra ; intros ; subst; by cbn in *. }
+    { by unfold regs_of; rewrite !dom_insert; set_solver+. }
+    iNext. iIntros (regs' retv) "(#Hspec & Hmem & Hreg)". iDestruct "Hspec" as %Hspec.
 
-   destruct Hspec as [ | | ]; try incrementPC_inv; simplify_map_eq; eauto.
-   { congruence. }
-   { iApply "Hφ". iFrame. rewrite insert_insert.
-     iDestruct (regs_of_map_3 with "Hmap") as "(?&?&?)"; eauto; iFrame. }
+   destruct Hspec as [ X | | | ]
+   ; [destruct X | | | ]
+   ; try (exfalso; simplify_map_eq; congruence)
+   ; match goal with | H: context[incrementPC _] |- _ => unfold incrementPC in H end
+   ; simplify_map_eq.
+   iApply "Hφ".
+   iExtractList "Hreg" [PC; r1;r2] as ["HPC";"Hr1";"Hr2"]; iFrame.
+   iDestruct (big_sepM_insert with "Hmem") as "[Hpc_a _]"; auto.
   Qed.
 
 End cap_lang_rules.
